init

HSM2FSM/Sub-goals/unique_fsm_state_names/case07.bpl
@@ -1,36 +1,18 @@
 implementation driver(){
-call init_tar_model(); 
-
-
-
-
+var s1: ref;
+var s2: ref;
+call init_tar_model();
+call RS2RS_matchAll();
 call IS2IS_matchAll();
-call IS2RS_matchAll();
-
-
+call RS2RS_applyAll();
 call IS2IS_applyAll();
-call IS2RS_applyAll();
-
-assert (
-
-forall s1:ref :: {read($tarHeap,s1,alloc)}
-  Seq#Contains(Fun#LIB#AllInstanceFrom($tarHeap, FSM$AbstractState), s1) ==>
-   genBy(s1, _IS2IS, $srcHeap, $tarHeap)  ==>
-    (forall s2: ref :: {read($tarHeap,s2,alloc)}
-      Seq#Contains(Fun#LIB#AllInstanceFrom($tarHeap, FSM$AbstractState), s2) ==>
-       genBy(s2, _IS2RS, $srcHeap, $tarHeap) ==>
-         s1 != s2 ==> read($tarHeap, s1, FSM$AbstractState.name) != read($tarHeap, s2, FSM$AbstractState.name))
-  
-) 
-;
-
-
+assume Seq#Contains(Fun#LIB#AllInstanceFrom($tarHeap, FSM$AbstractState), s2);
+assume genBy(s2, _RS2RS, $srcHeap, $tarHeap);
+assume s1 != s2;
+assume Seq#Contains(Fun#LIB#AllInstanceFrom($tarHeap, FSM$AbstractState), s1);
+assume genBy(s1, _IS2IS, $srcHeap, $tarHeap);
+assert genBy(s2, _RS2RS, $srcHeap, $tarHeap) || genBy(s2, _IS2IS, $srcHeap, $tarHeap) || genBy(s2, _IS2RS, $srcHeap, $tarHeap);
+assert genBy(s1, _RS2RS, $srcHeap, $tarHeap) || genBy(s1, _IS2IS, $srcHeap, $tarHeap) || genBy(s1, _IS2RS, $srcHeap, $tarHeap);
+assert read($tarHeap, s1, FSM$AbstractState.name) != read($tarHeap, s2, FSM$AbstractState.name);
 }
-
-
-
-
-
-
-  
 
