HSM2FSM/Sub-goals/fsm_state_multi_lower/case01.bpl
@@ -1,34 +1,16 @@
 implementation driver(){
-call init_tar_model(); 
-
-
+var s: ref;
+call init_tar_model();
 call SM2SM_matchAll();
-call RS2RS_matchAll();
-
-
+call IS2RS_matchAll();
 call SM2SM_applyAll();
-call RS2RS_applyAll();
-
-
-
-
-assert (
-
-forall s:ref :: {read($tarHeap,s,alloc)}
-  Seq#Contains(Fun#LIB#AllInstanceFrom($tarHeap, FSM$AbstractState), s)
-     ==> 
-     genBy(s, _RS2RS, $srcHeap, $tarHeap)
-     ==>
-     genBy(read($tarHeap, s, FSM$AbstractState.stateMachine), _SM2SM, $srcHeap, $tarHeap)
-     ==>
-     read($tarHeap, s, FSM$AbstractState.stateMachine)!=null
-  
-) 
-;
-
-
+call IS2RS_applyAll();
+assume Seq#Contains(Fun#LIB#AllInstanceFrom($tarHeap, FSM$AbstractState), s);
+assume !Seq#Contains(Fun#LIB#AllInstanceFrom($tarHeap, FSM$StateMachine), read($tarHeap, s, FSM$AbstractState.stateMachine));
+assume genBy(s, _IS2RS, $srcHeap, $tarHeap);
+assume read($tarHeap, s, FSM$AbstractState.stateMachine) == null || !read($tarHeap, read($tarHeap, s, FSM$AbstractState.stateMachine), alloc);
+assert genBy(s, _RS2RS, $srcHeap, $tarHeap) || genBy(s, _IS2IS, $srcHeap, $tarHeap) || genBy(s, _IS2RS, $srcHeap, $tarHeap);
+assert !(genBy(read($tarHeap, s, FSM$AbstractState.stateMachine), _SM2SM, $srcHeap, $tarHeap) || false);
+assert false;
 }
-
-
-
 
