HSM2FSM/Sub-goals/fsm_transition_multi_lower/case01.bpl
@@ -1,34 +1,16 @@
 implementation driver(){
-call init_tar_model(); 
-
-
+var t: ref;
+call init_tar_model();
 call SM2SM_matchAll();
-call T2TA_matchAll();
-
-
+call T2TB_matchAll();
 call SM2SM_applyAll();
-call T2TA_applyAll();
-
-
-
-
-
-assert (
-
-forall t:ref :: {read($tarHeap,t,alloc)}
-  Seq#Contains(Fun#LIB#AllInstanceFrom($tarHeap, FSM$Transition), t)
-  ==> 
-  genBy(t, _T2TA, $srcHeap, $tarHeap)
-  ==>
-  genBy(read($tarHeap, t, FSM$Transition.stateMachine), _SM2SM, $srcHeap, $tarHeap)
-  ==> 
-  read($tarHeap, t, FSM$Transition.stateMachine)!=null
-) 
-;
-
-
+call T2TB_applyAll();
+assume read($tarHeap, t, FSM$Transition.stateMachine) == null || !read($tarHeap, read($tarHeap, t, FSM$Transition.stateMachine), alloc);
+assume genBy(t, _T2TB, $srcHeap, $tarHeap);
+assume !Seq#Contains(Fun#LIB#AllInstanceFrom($tarHeap, FSM$StateMachine), read($tarHeap, t, FSM$Transition.stateMachine));
+assume Seq#Contains(Fun#LIB#AllInstanceFrom($tarHeap, FSM$Transition), t);
+assert !(genBy(read($tarHeap, t, FSM$Transition.stateMachine), _SM2SM, $srcHeap, $tarHeap) || false);
+assert genBy(t, _T2TA, $srcHeap, $tarHeap) || genBy(t, _T2TB, $srcHeap, $tarHeap) || genBy(t, _T2TC, $srcHeap, $tarHeap);
+assert false;
 }
-
-
-
 
