HSM2FSM/Sub-goals/fsm_transition_src_multi_lower/case07.bpl
@@ -1,39 +1,17 @@
 implementation driver(){
-call init_tar_model(); 
-
-
-
-
-call IS2RS_matchAll();
-
+var t: ref;
+call init_tar_model();
+call IS2IS_matchAll();
 call T2TB_matchAll();
-
-
-
-
-
-call IS2RS_applyAll();
-
+call IS2IS_applyAll();
 call T2TB_applyAll();
-
-
-
-assert  
-(
-
-forall t:ref :: {read($tarHeap,t,alloc)}
-  Seq#Contains(Fun#LIB#AllInstanceFrom($tarHeap, FSM$Transition), t) ==>
-    genBy(t, _T2TB, $srcHeap, $tarHeap) ==>
-      (
-
-      genBy(read($tarHeap, t, FSM$Transition.source), _IS2RS, $srcHeap, $tarHeap)  
-      )
-      ==>
-     read($tarHeap, t, FSM$Transition.source)!=null 
-) 
-;
-
-
-
-
+assume read($tarHeap, t, FSM$Transition.source) == null || !read($tarHeap, read($tarHeap, t, FSM$Transition.source), alloc);
+assume genBy(t, _T2TB, $srcHeap, $tarHeap);
+assume Seq#Contains(Fun#LIB#AllInstanceFrom($tarHeap, FSM$Transition), t);
+assume Seq#Contains(Fun#LIB#AllInstanceFrom($tarHeap, FSM$AbstractState), read($tarHeap, t, FSM$Transition.source));
+assume genBy(read($tarHeap, t, FSM$Transition.source), _IS2IS, $srcHeap, $tarHeap);
+assert genBy(t, _T2TA, $srcHeap, $tarHeap) || genBy(t, _T2TB, $srcHeap, $tarHeap) || genBy(t, _T2TC, $srcHeap, $tarHeap);
+assert genBy(read($tarHeap, t, FSM$Transition.source), _RS2RS, $srcHeap, $tarHeap) || genBy(read($tarHeap, t, FSM$Transition.source), _IS2IS, $srcHeap, $tarHeap) || genBy(read($tarHeap, t, FSM$Transition.source), _IS2RS, $srcHeap, $tarHeap);
+assert false;
 }
+
