HSM2FSM/Sub-goals/fsm_transition_trg_multi_lower/case11.bpl
@@ -1,38 +1,17 @@
 implementation driver(){
-call init_tar_model(); 
-
-
-
+var t: ref;
+call init_tar_model();
 call IS2RS_matchAll();
-
 call T2TC_matchAll();
-
-
-
-
 call IS2RS_applyAll();
-
 call T2TC_applyAll();
-
-
-assert (forall t:ref :: {read($tarHeap,t,alloc)}
-  Seq#Contains(Fun#LIB#AllInstanceFrom($tarHeap, FSM$Transition), t) ==>   
-    (
-    genBy(t, _T2TC, $srcHeap, $tarHeap)
-    )
-     ==> 
-     (
-
-      genBy(read($tarHeap, t, FSM$Transition.target), _IS2RS, $srcHeap, $tarHeap) 
-     )
-     ==>
-     read($tarHeap, t, FSM$Transition.target)!=null
-    
-) ;
-
-
+assume Seq#Contains(Fun#LIB#AllInstanceFrom($tarHeap, FSM$AbstractState), read($tarHeap, t, FSM$Transition.target));
+assume read($tarHeap, t, FSM$Transition.target) == null || !read($tarHeap, read($tarHeap, t, FSM$Transition.target), alloc);
+assume genBy(read($tarHeap, t, FSM$Transition.target), _IS2RS, $srcHeap, $tarHeap);
+assume Seq#Contains(Fun#LIB#AllInstanceFrom($tarHeap, FSM$Transition), t);
+assume genBy(t, _T2TC, $srcHeap, $tarHeap);
+assert genBy(read($tarHeap, t, FSM$Transition.target), _RS2RS, $srcHeap, $tarHeap) || genBy(read($tarHeap, t, FSM$Transition.target), _IS2IS, $srcHeap, $tarHeap) || genBy(read($tarHeap, t, FSM$Transition.target), _IS2RS, $srcHeap, $tarHeap);
+assert genBy(t, _T2TA, $srcHeap, $tarHeap) || genBy(t, _T2TB, $srcHeap, $tarHeap) || genBy(t, _T2TC, $srcHeap, $tarHeap);
+assert false;
 }
-
-
-
 
